Найдём интеграл, вида
\begin{equation*}
    I_n = \int_{0}^{\infty}  \frac{J_n (z)}{z^n} \d z.
\end{equation*}
Вспомним, что
\begin{equation*}
    \partial_z \left(z^m J_m[z]\right) = z^m J_{m-1}[z],
    \hspace{5 mm} 
    \text{или}
    \hspace{5 mm} 
    J_m [z] = \frac{1}{z^{m+1}} \partial_z \left(z^{m+1} J_{m+1}[z]\right).
\end{equation*}
Подставляя в $I_n$, и, интегрируя по частям, находим
\begin{equation*}
    I_n (z) = \frac{J_{n+1}}{z^n} \bigg|_0^{\infty} - \int_{0}^{+\infty} z^{n+1} J_{n+1} \frac{-2n-1}{z^{2n+2}} \d z = (2n + 1) \int_{0}^{\infty} \frac{J_{n+1}}{z^{n+1}} \d z = (2n + 1) I_{n+1},
\end{equation*}
откуда
\begin{equation*}
    I_n = \frac{1}{(2n-1)!!} I_0.
\end{equation*}
Осталось найти $I_0$, как, например, $\Lambda[J_0](1)$:
\begin{equation*}
    I_0 = \int_{0}^{\infty} J_0  (z) \d z =
    \int_{0}^{\infty} J_0  (z) \d z = \Lambda[J_0](0) = 1,
\end{equation*}
а значит исходный интеграл:
\begin{equation*}
    I_n = \int_{0}^{\infty}  \frac{J_n (z)}{z^n} \d z = \frac{1}{(2n-1)!!},
    \hspace{10 mm} 
    I_2 = \frac{1}{3}.
\end{equation*}