\section{Неделя VII}

\subsection*{№1 (3.2.1)}

Известно, что 
\begin{equation*}
    \Ai (x) = \frac{1}{\pi} \int_{0}^{\infty} \cos\left(x u + \frac{u^3}{3}\right) \d u,
    \hspace{10 mm} 
    \Bi(x) = \frac{1}{\pi} \int_{0}^{\infty} \left[
        \exp\left(x u - \frac{u^3}{3}\right) + \sin\left(x u + \frac{u^3}{3}\right)
    \right] \d u.
\end{equation*}
Найдём значения в $x = 0$, переходя к $u = t^{1/3}$:
\begin{equation*}
    \Ai(0) = \frac{1}{\pi} \int_{0}^{\infty} \cos( u^3/3) \d u = 
    \frac{1}{\pi} \int_{0}^{\infty} \frac{\cos(t/3) }{3 t^{2/3}}\d t = \frac{1}{3^{2/3} \Gamma\left(\frac{2}{3}\right)}.
\end{equation*}
Аналогично для $\Bi$:
\begin{equation*}
    \Bi(0) = \frac{1}{\pi} \int_{0}^{\infty} \left[
        \exp\left( - u^3/3\right) + \sin( u^3/3)
    \right] \d u = 
    \frac{1}{\pi} \int_{0}^{\infty} \frac{e^{-\frac{t}{3}}+\sin \left(\frac{t}{3}\right)}{3 t^{2/3}} \d t =  
    \frac{\Gamma \left(\frac{1}{3}\right)}{3^{2/3} \pi } -\frac{\Gamma \left(-\frac{2}{3}\right)}{3^{5/3} \pi } = \frac{1}{3^{1/6} \Gamma\left(\frac{2}{3}\right)}.
\end{equation*}

Теперь, дифференцируя под знаком интеграла, находим
\begin{equation*}
    \Ai'(0) = 
    \frac{1}{\pi} \int_{0}^{\infty} 
    -\frac{\sin \left(\frac{t}{3}\right)}{3 \sqrt[3]{t}}
    \d t = -\frac{1}{\sqrt[3]{3} \Gamma \left(\frac{1}{3}\right)}.
\end{equation*}
Аналогично для $\Bi$:
\begin{equation*}
    \Bi'(0) = 
    \frac{1}{\pi} \int_{0}^{\infty} 
    \left(
        \frac{e^{-\frac{t}{3}}}{3 \sqrt[3]{t}}+\frac{\cos \left(\frac{t}{3}\right)}{3 \sqrt[3]{t}}
    \right)
    \d t = \frac{\Gamma \left(\frac{2}{3}\right)}{\sqrt[3]{3} \pi } + \frac{\Gamma \left(\frac{2}{3}\right)}{2 \sqrt[3]{3} \pi } = \frac{3^{2/3} \Gamma \left(\frac{2}{3}\right)}{2 \pi } = \frac{3^{1/6}}{\Gamma\left(\frac{1}{3}\right)}.
\end{equation*}