Найдём значение интеграла 
\begin{equation*}
    I_n = \int_{-\infty}^{+\infty} \exp(-(x-y)^2) H_n (x) \d x.
\end{equation*}
Вспоминая, что
\begin{equation*}
    H_n (x) = (-1)^n e^{x^2} \partial_x^n e^{-x^2},
\end{equation*}
переписываем $I_n$, как
\begin{equation*}
    I_n = (-1)^n e^{-y^2} \int_{-\infty}^{+\infty}  e^{2 xy} \partial_x^n e^{-x^2} \d x = e^{-y^2} \int_{-\infty}^{+\infty} 2^n y^n e^{2xy} e^{-x^2} \d x = 2^n y^n \sqrt{\pi},
\end{equation*}
где мы просто много раз проинтегрировали по частям. Итого, исходный интеграл:
\begin{equation*}
    I_n =\int_{-\infty}^{+\infty} \exp(-(x-y)^2) H_n (x) \d x= 2^n y^n \sqrt{\pi}.
\end{equation*}